src/Std/Data/DTreeMap/Basic.lean
@@ -250,11 +250,7 @@ def fromArray (l : Array ((a : α) × β a)) (cmp : α → α → Ordering) : DT
 
 @[inline, inherit_doc Raw.mergeBy]
 def mergeBy [LawfulEqCmp cmp] (mergeFn : (a : α) → β a → β a → β a) (t₁ t₂ : DTreeMap α β cmp) : DTreeMap α β cmp :=
-  t₂.foldl (init := t₁) fun t₁ a b₂ =>
-    t₁.insert a <|
-      match t₁.get? a with
-      | some b₁ => mergeFn a b₁ b₂
-      | none => b₂
+  letI : Ord α := ⟨cmp⟩; ⟨t₁.inner.mergeBy mergeFn t₂.inner t₁.wf.balanced |>.impl, sorry⟩
 
 namespace Const
 
@@ -287,11 +283,8 @@ def fromArray (l : Array (α × β)) (cmp : α → α → Ordering) : DTreeMap �
 
 @[inline, inherit_doc Raw.Const.mergeBy]
 def mergeBy (mergeFn : α → β → β → β) (t₁ t₂ : DTreeMap α β cmp) : DTreeMap α β cmp :=
-  t₂.foldl (init := t₁) fun t₁ a b₂ =>
-    t₁.insert a <|
-      match get? t₁ a with
-      | some b₁ => mergeFn a b₁ b₂
-      | none => b₂
+  letI : Ord α := ⟨cmp⟩;
+  ⟨Impl.Const.mergeBy mergeFn t₁.inner t₂.inner t₁.wf.balanced |>.impl, sorry⟩
 
 end Const
 
